HoareAsLogic.v
@@ -1,0 +1,201 @@
+Add LoadPath "D:\sfsol".
+Require Export Hoare.
+
+Inductive hoare_proof : Assertion -> com -> Assertion -> Type :=
+  | H_Skip : forall P,
+      hoare_proof P (SKIP) P
+  | H_Asgn : forall Q V a,
+      hoare_proof (assn_sub V a Q) (V ::= a) Q
+  | H_Seq : forall P c Q d R,
+      hoare_proof P c Q -> hoare_proof Q d R -> hoare_proof P (c;;d) R
+  | H_If : forall P Q b c1 c2,
+    hoare_proof (fun st => P st /\ bassn b st) c1 Q ->
+    hoare_proof (fun st => P st /\ ~(bassn b st)) c2 Q ->
+    hoare_proof P (IFB b THEN c1 ELSE c2 FI) Q
+  | H_While : forall P b c,
+    hoare_proof (fun st => P st /\ bassn b st) c P ->
+    hoare_proof P (WHILE b DO c END) (fun st => P st /\ ~ (bassn b st))
+  | H_Consequence : forall (P Q P' Q' : Assertion) c,
+    hoare_proof P' c Q' ->
+    (forall st, P st -> P' st) ->
+    (forall st, Q' st -> Q st) ->
+    hoare_proof P c Q.
+
+Tactic Notation "hoare_proof_cases" tactic(first) ident(c) :=
+  first;
+  [ Case_aux c "H_Skip" | Case_aux c "H_Asgn" | Case_aux c "H_Seq"
+  | Case_aux c "H_If" | Case_aux c "H_While" | Case_aux c "H_Consequence" ].
+
+Lemma H_Consequence_pre : forall (P Q P': Assertion) c,
+    hoare_proof P' c Q ->
+    (forall st, P st -> P' st) ->
+    hoare_proof P c Q.
+Proof.
+  intros.
+  eapply H_Consequence.
+  apply X. assumption. auto.
+  Qed.
+
+Lemma H_Consequence_post : forall (P Q Q': Assertion) c,
+    hoare_proof P c Q' ->
+    (forall st, Q' st -> Q st) ->
+    hoare_proof P c Q.
+Proof.
+  intros.
+  eapply H_Consequence.
+  apply X. auto. assumption.
+  Qed.
+
+Example sample_proof
+             : hoare_proof
+                 (assn_sub X (APlus (AId X) (ANum 1))
+                   (assn_sub X (APlus (AId X) (ANum 2))
+                     (fun st => st X = 3) ))
+                 (X ::= APlus (AId X) (ANum 1);; (X ::= APlus (AId X) (ANum 2)))
+                 (fun st => st X = 3).
+Proof.
+  eapply H_Seq; apply H_Asgn.
+Qed.
+
+Theorem hoare_proof_sound : forall P c Q,
+  hoare_proof P c Q -> {{P}} c {{Q}}.
+Proof.
+  intros. induction X.
+  apply hoare_skip.
+  apply hoare_asgn.
+  apply hoare_seq with Q; assumption.
+  apply hoare_if; assumption.
+  apply hoare_while; assumption.
+  eapply hoare_consequence; try apply IHX; try assumption.
+  Qed.
+
+Theorem H_Post_True_deriv:
+  forall c P, hoare_proof P c (fun _ => True).
+Proof.
+  intro c.
+  com_cases (induction c) Case; intro P.
+  Case "SKIP".
+    eapply H_Consequence.
+    apply H_Skip.
+    intros. apply H.
+    (* Proof of True *)
+    intros. apply I.
+  Case "::=".
+    eapply H_Consequence_pre.
+    apply H_Asgn.
+    intros. apply I.
+  Case ";;".
+    eapply H_Consequence_pre.
+    eapply H_Seq.
+    apply (IHc1 (fun _ => True)).
+    apply IHc2.
+    intros. apply I.
+  Case "IFB".
+    apply H_Consequence_pre with (fun _ => True).
+    apply H_If.
+    apply IHc1.
+    apply IHc2.
+    intros. apply I.
+  Case "WHILE".
+    eapply H_Consequence.
+    eapply H_While.
+    eapply IHc.
+    intros; apply I.
+    intros; apply I.
+Qed.
+
+Lemma False_and_P_imp: forall P Q,
+  False /\ P -> Q.
+Proof.
+  intros P Q [CONTRA HP].
+  destruct CONTRA.
+Qed.
+
+Tactic Notation "pre_false_helper" constr(CONSTR) :=
+  eapply H_Consequence_pre;
+    [eapply CONSTR | intros ? CONTRA; destruct CONTRA].
+
+Theorem H_Pre_False_deriv:
+  forall c Q, hoare_proof (fun _ => False) c Q.
+Proof.
+  intros c.
+  com_cases (induction c) Case; intro Q.
+  Case "SKIP". pre_false_helper H_Skip.
+  Case "::=". pre_false_helper H_Asgn.
+  Case ";;". pre_false_helper H_Seq. apply IHc1. apply IHc2.
+  Case "IFB".
+    apply H_If; eapply H_Consequence_pre.
+    apply IHc1. intro. eapply False_and_P_imp.
+    apply IHc2. intro. eapply False_and_P_imp.
+  Case "WHILE".
+    eapply H_Consequence_post.
+    eapply H_While.
+    eapply H_Consequence_pre.
+      apply IHc.
+      intro. eapply False_and_P_imp.
+    intro. simpl. eapply False_and_P_imp.
+Qed.
+
+Definition wp (c:com) (Q:Assertion) : Assertion :=
+  fun s => forall s', c / s || s' -> Q s'.
+
+Lemma wp_is_precondition: forall c Q,
+  {{wp c Q}} c {{Q}}.
+Proof.
+  intros c Q st st' H1 H2.
+  apply H2. assumption.
+  Qed.
+
+Lemma wp_is_weakest: forall c Q P',
+   {{P'}} c {{Q}} -> forall st, P' st -> wp c Q st.
+Proof.
+  intros c Q P' H st H2. unfold wp. intros s' Hypo.
+  eapply H. apply Hypo. assumption. Qed.
+
+Lemma bassn_eval_false : forall b st, ~ bassn b st -> beval st b = false.
+Proof.
+  intros b st H. unfold bassn in H. destruct (beval st b).
+    exfalso. apply H. reflexivity.
+    reflexivity.
+Qed.
+
+Theorem hoare_proof_complete: forall P c Q,
+  {{P}} c {{Q}} -> hoare_proof P c Q.
+Proof.
+  intros P c. generalize dependent P.
+  com_cases (induction c) Case; intros P Q HT.
+  Case "SKIP".
+    eapply H_Consequence.
+     eapply H_Skip.
+      intros. eassumption.
+      intro st. apply HT. apply E_Skip.
+  Case "::=".
+    eapply H_Consequence.
+      eapply H_Asgn.
+      intro st. apply HT. econstructor. reflexivity.
+      intros; assumption.
+  Case ";;".
+    apply H_Seq with (wp c2 Q).
+     eapply IHc1.
+       intros st st' E1 H. unfold wp. intros st'' E2.
+         eapply HT. econstructor; eassumption. assumption.
+     eapply IHc2. intros st st' E1 H. apply H; assumption.
+  Case "IFB".
+    apply H_If. apply IHc1.
+      intros st st' H [H1 H2].
+      eapply HT. constructor; try apply H2; assumption. assumption.
+      apply IHc2. intros st st' H [H1 H2].
+      eapply HT. apply E_IfFalse; try apply bassn_eval_false; try apply H2; assumption. assumption.
+  Case "WHILE".
+    eapply H_Consequence with (P' := wp (WHILE b DO c END) Q).
+      apply H_While.
+      apply IHc. intros st st' H [H2 H3] st'' H4.
+      assert((WHILE b DO c END) / st || st'').
+        eapply E_WhileLoop. apply H3. apply H. apply H4.
+      eapply wp_is_precondition. apply H0. assumption.
+      apply wp_is_weakest. assumption.
+      intros st [H1 H2]. eapply wp_is_precondition.
+      assert((WHILE b DO c END) / st || st).
+        apply E_WhileEnd. apply bassn_eval_false. assumption.
+      apply H. assumption.
+  Qed.
