HoareList.v
@@ -1,0 +1,883 @@
+Add LoadPath "D:\sfsol".
+Require Export SfLib.
+
+Inductive id : Type := 
+  Id : nat -> id.
+
+Theorem eq_id_dec : forall id1 id2 : id, {id1 = id2} + {id1 <> id2}.
+Proof.
+   intros id1 id2.
+   destruct id1 as [n1]. destruct id2 as [n2].
+   destruct (eq_nat_dec n1 n2) as [Heq | Hneq].
+   Case "n1 = n2".
+     left. rewrite Heq. reflexivity.
+   Case "n1 <> n2".
+     right. intros contra. inversion contra. apply Hneq. apply H0.
+Defined. 
+
+Lemma eq_id : forall (T:Type) x (p q:T), 
+              (if eq_id_dec x x then p else q) = p. 
+Proof.
+  intros. 
+  destruct (eq_id_dec x x). 
+  Case "x = x". 
+    reflexivity.
+  Case "x <> x (impossible)". 
+    apply ex_falso_quodlibet; apply n; reflexivity. Qed.
+
+Lemma neq_id : forall (T:Type) x y (p q:T), x <> y -> 
+               (if eq_id_dec x y then p else q) = q. 
+Proof.
+  intros. 
+  destruct (eq_id_dec x y). 
+  Case "x = y (impossible)". 
+    subst. apply ex_falso_quodlibet; apply H; reflexivity.
+  Case "x <> y". 
+    reflexivity. Qed.
+
+Definition X : id := Id 0.
+Definition Y : id := Id 1.
+Definition Z : id := Id 2.
+
+Inductive val : Type :=
+| VNat : nat -> val
+| VList : list nat -> val.
+
+Definition state := id -> val.
+
+Definition empty_state : state := fun _ => VNat 0.
+Definition update (st : state) (X:id) (v : val) : state :=
+  fun X' => if eq_id_dec X X' then v else st X'.
+
+Definition asnat (v : val) : nat :=
+  match v with
+  | VNat n => n
+  | VList _ => 0
+  end.
+
+Definition aslist (v : val) : list nat :=
+  match v with
+  | VNat n => []
+  | VList xs => xs
+  end.
+
+Inductive aexp : Type := 
+  | ANum : nat -> aexp
+  | AId : id -> aexp
+  | APlus : aexp -> aexp -> aexp
+  | AMinus : aexp -> aexp -> aexp
+  | AMult : aexp -> aexp -> aexp
+  | AHead : aexp -> aexp
+  | ATail : aexp -> aexp
+  | ACons : aexp -> aexp -> aexp
+  | ANil  : aexp.
+
+Tactic Notation "aexp_cases" tactic(first) ident(c) :=
+  first;
+  [ Case_aux c "ANum" | Case_aux c "AId" | Case_aux c "APlus"
+  | Case_aux c "AMinus" | Case_aux c "AMult"
+  | Case_aux c "AHead" | Case_aux c "ATail"
+  | Case_aux c "ACons" | Case_aux c "ANil" ].
+
+Definition tail (l : list nat) :=
+  match l with
+  | x::xs => xs
+  | [] => []
+  end.
+
+Definition head (l : list nat) :=
+  match l with
+  | x::xs => x
+  | [] => 0
+  end.
+
+Fixpoint aeval (st : state) (e : aexp) : val :=
+  match e with
+  | ANum n => VNat n
+  | AId i => st i
+  | APlus a1 a2   => VNat (asnat (aeval st a1) + asnat (aeval st a2))
+  | AMinus a1 a2  => VNat (asnat (aeval st a1) - asnat (aeval st a2))
+  | AMult a1 a2   => VNat (asnat (aeval st a1) * asnat (aeval st a2))
+  | ATail a => VList (tail (aslist (aeval st a)))
+  | AHead a => VNat (head (aslist (aeval st a)))
+  | ACons a1 a2 => VList (asnat (aeval st a1) :: aslist (aeval st a2))
+  | ANil => VList []
+  end. 
+
+Inductive bexp : Type := 
+  | BTrue : bexp
+  | BFalse : bexp
+  | BEq : aexp -> aexp -> bexp
+  | BLe : aexp -> aexp -> bexp
+  | BNot : bexp -> bexp
+  | BAnd : bexp -> bexp -> bexp
+  | BIsCons : aexp -> bexp.
+
+Tactic Notation "bexp_cases" tactic(first) ident(c) :=
+  first;
+  [ Case_aux c "BTrue" | Case_aux c "BFalse" | Case_aux c "BEq"
+  | Case_aux c "BLe" | Case_aux c "BNot" | Case_aux c "BAnd"
+  | Case_aux c "BIsCons" ].
+
+Fixpoint beval (st : state) (e : bexp) : bool :=
+  match e with 
+  | BTrue       => true
+  | BFalse      => false
+  | BEq a1 a2   => beq_nat (asnat (aeval st a1)) (asnat (aeval st a2))
+  | BLe a1 a2   => ble_nat (asnat (aeval st a1)) (asnat (aeval st a2))
+  | BNot b1     => negb (beval st b1)
+  | BAnd b1 b2  => andb (beval st b1) (beval st b2)
+  | BIsCons a    => match aslist (aeval st a) with
+                     | _::_ => true
+                     | [] => false
+                   end
+  end.
+
+Theorem update_eq : forall n V st,
+  (update st V n) V = n.
+Proof.
+  intros n V st.
+  unfold update.
+  rewrite eq_id. 
+  reflexivity.
+Qed.
+
+Theorem update_neq : forall V2 V1 n st,
+  V2 <> V1 -> 
+  (update st V2 n) V1 = (st V1).
+Proof.
+  intros V2 V1 n st Hneq.
+  unfold update.
+  rewrite neq_id. 
+  reflexivity. 
+  assumption. Qed.
+
+Theorem update_shadow : forall x1 x2 k1 k2 (f : state),
+   (update  (update f k2 x1) k2 x2) k1 = (update f k2 x2) k1.
+Proof.
+  intros x1 x2 k1 k2 f.
+  unfold update.
+  destruct (eq_id_dec k2 k1); reflexivity.  Qed.
+
+Theorem update_same : forall x1 k1 k2 (f : state),
+  f k1 = x1 ->
+  (update f k1 x1) k2 = f k2.
+Proof.
+  intros x1 k1 k2 f Heq.
+  unfold update. subst.
+  destruct (eq_id_dec k1 k2). 
+  Case "k1 = k2".
+    subst. reflexivity.
+  Case "k1 <> k2".
+    reflexivity.  Qed.
+
+Theorem update_permute : forall x1 x2 k1 k2 k3 f,
+  k2 <> k1 -> 
+  (update (update f k2 x1) k1 x2) k3 = (update (update f k1 x2) k2 x1) k3.
+Proof.
+  intros x1 x2 k1 k2 k3 f H.
+  unfold update.
+  destruct (eq_id_dec k1 k3); try reflexivity.
+  Case "k1 = k3".
+      subst. rewrite neq_id. reflexivity. assumption. Qed.
+
+Inductive com : Type :=
+  | CSkip : com
+  | CAss : id -> aexp -> com
+  | CSeq : com -> com -> com
+  | CIf : bexp -> com -> com -> com
+  | CWhile : bexp -> com -> com.
+
+Tactic Notation "com_cases" tactic(first) ident(c) :=
+  first;
+  [ Case_aux c "SKIP" | Case_aux c "::=" | Case_aux c ";"
+  | Case_aux c "IFB" | Case_aux c "WHILE" ].
+
+Notation "'SKIP'" := 
+  CSkip.
+Notation "X '::=' a" := 
+  (CAss X a) (at level 60).
+Notation "c1 ; c2" := 
+  (CSeq c1 c2) (at level 80, right associativity).
+Notation "'WHILE' b 'DO' c 'END'" := 
+  (CWhile b c) (at level 80, right associativity).
+Notation "'IFB' e1 'THEN' e2 'ELSE' e3 'FI'" := 
+  (CIf e1 e2 e3) (at level 80, right associativity).
+
+Reserved Notation "c1 '/' st '||' st'" (at level 40, st at level 39).
+
+Inductive ceval : state -> com -> state -> Prop :=
+  | E_Skip : forall st,
+      SKIP / st || st
+  | E_Asgn  : forall st a1 n X,
+      aeval st a1 = n ->
+      (X ::= a1) / st || (update st X n)
+  | E_Seq : forall c1 c2 st st' st'',
+      c1 / st  || st' ->
+      c2 / st' || st'' ->
+      (c1 ; c2) / st || st''
+  | E_IfTrue : forall st st' b1 c1 c2,
+      beval st b1 = true ->
+      c1 / st || st' ->
+      (IFB b1 THEN c1 ELSE c2 FI) / st || st'
+  | E_IfFalse : forall st st' b1 c1 c2,
+      beval st b1 = false ->
+      c2 / st || st' ->
+      (IFB b1 THEN c1 ELSE c2 FI) / st || st'
+  | E_WhileEnd : forall b1 st c1,
+      beval st b1 = false ->
+      (WHILE b1 DO c1 END) / st || st
+  | E_WhileLoop : forall st st' st'' b1 c1,
+      beval st b1 = true ->
+      c1 / st || st' ->
+      (WHILE b1 DO c1 END) / st' || st'' ->
+      (WHILE b1 DO c1 END) / st || st''
+
+  where "c1 '/' st '||' st'" := (ceval st c1 st').
+
+Tactic Notation "ceval_cases" tactic(first) ident(c) :=
+  first;
+  [ Case_aux c "E_Skip" | Case_aux c "E_Asgn" | Case_aux c "E_Seq"
+  | Case_aux c "E_IfTrue" | Case_aux c "E_IfFalse"
+  | Case_aux c "E_WhileEnd" | Case_aux c "E_WhileLoop" ].
+
+Definition Assertion := state -> Prop.
+
+Definition hoare_triple (P:Assertion) (c:com) (Q:Assertion) : Prop :=
+  forall st st', 
+       c / st || st'  ->
+       P st  ->
+       Q st'.
+
+Notation "{{ P }}  c  {{ Q }}" := (hoare_triple P c Q) 
+                                  (at level 90, c at next level) 
+                                  : hoare_spec_scope.
+Open Scope hoare_spec_scope.
+
+Definition assn_sub X a Q : Assertion :=
+  fun (st : state) =>
+    Q (update st X (aeval st a)).
+
+Theorem hoare_asgn : forall Q X a,
+  {{assn_sub X a Q}} (X ::= a) {{Q}}.
+Proof.
+  unfold hoare_triple.
+  intros Q X a st st' HE HQ.
+  inversion HE. subst.
+  unfold assn_sub in HQ. assumption.  Qed.
+
+Theorem hoare_skip : forall P,
+     {{P}} SKIP {{P}}.
+Proof.
+  intros P st st' H HP. inversion H. subst.
+  assumption.  Qed.
+
+Theorem hoare_seq : forall P Q R c1 c2,
+     {{Q}} c2 {{R}} ->
+     {{P}} c1 {{Q}} ->
+     {{P}} c1;c2 {{R}}.
+Proof.
+  intros P Q R c1 c2 H1 H2 st st' H12 Pre.
+  inversion H12; subst.
+  apply (H1 st'0 st'); try assumption.
+  apply (H2 st st'0); assumption. Qed.
+
+Definition bassn b : Assertion :=
+  fun st => (beval st b = true).
+
+Lemma bexp_eval_true : forall b st,
+  beval st b = true -> (bassn b) st.
+Proof.
+  intros b st Hbe.
+  unfold bassn. assumption.  Qed.
+
+Lemma bexp_eval_false : forall b st,
+  beval st b = false -> ~ ((bassn b) st).
+Proof.
+  intros b st Hbe contra.
+  unfold bassn in contra.
+  rewrite -> contra in Hbe. inversion Hbe.  Qed.
+
+Theorem hoare_if : forall P Q b c1 c2,
+  {{fun st => P st /\ bassn b st}} c1 {{Q}} ->
+  {{fun st => P st /\ ~(bassn b st)}} c2 {{Q}} ->
+  {{P}} (IFB b THEN c1 ELSE c2 FI) {{Q}}.
+Proof.
+  intros P Q b c1 c2 HTrue HFalse st st' HE HP.
+  inversion HE; subst. 
+  Case "b is true".
+    apply (HTrue st st'). 
+      assumption. 
+      split. assumption. 
+             apply bexp_eval_true. assumption.
+  Case "b is false".
+    apply (HFalse st st'). 
+      assumption. 
+      split. assumption.
+             apply bexp_eval_false. assumption. Qed.
+
+Lemma hoare_while : forall P b c,
+  {{fun st => P st /\ bassn b st}} c {{P}} ->
+  {{P}} WHILE b DO c END {{fun st => P st /\ ~ (bassn b st)}}.
+Proof.
+  intros P b c Hhoare st st' He HP.
+  remember (WHILE b DO c END) as wcom.
+  ceval_cases (induction He) Case; try (inversion Heqwcom); subst.
+  
+  Case "E_WhileEnd".
+    split. assumption. apply bexp_eval_false.  assumption.
+
+  Case "E_WhileLoop".
+    apply IHHe2.  reflexivity.
+    apply (Hhoare st st'); try assumption.
+      split. assumption. apply bexp_eval_true. assumption.  Qed.
+
+Definition assert_implies (P Q : Assertion) : Prop :=
+  forall st, P st -> Q st.
+
+Notation "P ->> Q" := (assert_implies P Q) (at level 80).
+Notation "P <<->> Q" := (P ->> Q /\ Q ->> P) (at level 80).
+
+Theorem hoare_consequence_pre : forall (P P' Q : Assertion) c,
+  {{P'}} c {{Q}} ->
+  P ->> P' ->
+  {{P}} c {{Q}}.
+Proof.
+  intros P P' Q c Hhoare Himp.
+  intros st st' Hc HP. apply (Hhoare st st'). 
+  assumption. apply Himp. assumption. Qed.
+
+Theorem hoare_consequence_post : forall (P Q Q' : Assertion) c,
+  {{P}} c {{Q'}} ->
+  Q' ->> Q ->
+  {{P}} c {{Q}}.
+Proof.
+  intros P Q Q' c Hhoare Himp.
+  intros st st' Hc HP. 
+  apply Himp.
+  apply (Hhoare st st'). 
+  assumption. assumption. Qed.
+
+Theorem hoare_consequence : forall (P P' Q Q' : Assertion) c,
+  {{P'}} c {{Q'}} ->
+  P ->> P' ->
+  Q' ->> Q ->
+  {{P}} c {{Q}}.
+Proof.
+  intros P P' Q Q' c Hht HPP' HQ'Q.
+  intros st st' Hc HP.
+  apply HQ'Q. apply (Hht st st'). assumption.
+  apply HPP'. assumption. Qed.
+
+Definition list_member :=
+  WHILE BIsCons (AId X) DO
+    IFB (BEq (AId Y) (AHead (AId X))) THEN
+      Z ::= (ANum 1)
+    ELSE
+      SKIP
+    FI;
+    X ::= ATail (AId X)
+  END.
+
+Fixpoint snoc {X:Type} (l:list X) (v:X) : (list X) :=
+  match l with
+  | nil => [ v ]
+  | cons h t => h :: (snoc t v)
+  end.
+
+Lemma snoc_equation : forall (A : Type) (h:A) (x y : list A),
+  snoc x h ++ y = x ++ h :: y.     
+Proof.
+  intros A h x y.
+  induction x. 
+    Case "x = []". reflexivity.
+    Case "x = cons". simpl. rewrite IHx. reflexivity.
+Qed.
+
+Lemma appears_in_snoc1 : forall a l,
+  appears_in a (snoc l a).
+Proof.
+  induction l.
+    Case "l = []". apply ai_here.
+    Case "l = cons". simpl. apply ai_later. apply IHl.
+Qed.
+
+Lemma appears_in_snoc2 : forall a b l,
+  appears_in a l ->
+  appears_in a (snoc l b).
+Proof.
+  induction l; intros H; inversion H; subst; simpl.
+    Case "l = []". apply ai_here.
+    Case "l = cons". apply ai_later. apply IHl. assumption.
+Qed.
+
+Lemma appears_in_snoc3 : forall a b l,
+   appears_in a (snoc l b) ->
+   (appears_in a l \/ a = b).
+Proof.
+   induction l; intros H.
+   Case "l = []". inversion H.
+     SCase "ai_here". right. reflexivity.
+     SCase "ai_later". left. assumption.
+   Case "l = cons". inversion H; subst.
+     SCase "ai_here". left. apply ai_here.
+     SCase "ai_later". destruct (IHl H1).
+       left. apply ai_later. assumption.
+       right. assumption.
+Qed.
+
+Lemma append_singleton_equation : forall (x : nat) l l',
+  (l ++ [x]) ++ l' = l ++ x :: l'.
+Proof.
+  intros x l l'.
+  induction l.
+    reflexivity.
+    simpl. rewrite IHl. reflexivity.
+Qed.
+
+Lemma append_nil : forall (A : Type) (l : list A),
+  l ++ [] = l.
+Proof.
+  induction l. 
+    reflexivity.
+    simpl. rewrite IHl. reflexivity.
+Qed.
+
+Theorem list_member_correct : forall l n,
+  {{ fun st => aslist (st X) = l /\ asnat (st Y) = n /\ asnat (st Z) = 0 }}
+  list_member
+  {{ fun st => asnat (st Z) = 1 <-> appears_in n l }}.
+Proof.
+  intros l n.
+  eapply hoare_consequence.
+  apply hoare_while with (P := fun st =>
+     asnat (st Y) = n 
+     /\ exists p, p ++ aslist (st X) = l 
+                  /\ (asnat (st Z) = 1 <-> appears_in n p)).
+    (* The loop body preserves the invariant: *)
+    eapply hoare_seq.
+    apply hoare_asgn.
+    apply hoare_if.
+    Case "If taken".
+      eapply hoare_consequence_pre.
+      apply hoare_asgn.
+      intros st [[[H1 [p [H2 H3]]] H9] H10].
+      unfold assn_sub. split.
+      (* (st Y) is still n *)
+        rewrite update_neq; try (intro X; inversion X). 
+        rewrite update_neq; try (intro X; inversion X). 
+        assumption.
+      (* and the interesting part of the invariant is preserved: *)
+        (* X has to be a cons *)
+        destruct (aslist (st X)) as [|h x'] eqn:Heqx. 
+          unfold bassn in H9. unfold beval in H9. unfold aeval in H9. 
+          rewrite -> Heqx in H9. inversion H9.
+          
+          exists (snoc p h).
+          rewrite update_eq.
+          unfold aeval. rewrite update_neq; try (intro X; inversion X). 
+          rewrite -> Heqx.
+          split.
+            rewrite snoc_equation. assumption.
+
+            rewrite update_neq; try (intro X; inversion X). 
+            rewrite update_eq. 
+            split. 
+              simpl.
+              unfold bassn in H10. unfold beval in H10.
+              unfold aeval in H10. rewrite H1 in H10. 
+              rewrite -> Heqx in H10. simpl in H10.
+              rewrite (beq_nat_true _ _ H10).
+              intros. apply appears_in_snoc1.
+                
+              intros. reflexivity.
+    Case "If not taken".
+      eapply hoare_consequence_pre. apply hoare_skip.
+      unfold assn_sub.
+      intros st [[[H1 [p [H2 H3]]] H9] H10].
+      split.
+      (* (st Y) is still n *)
+        rewrite update_neq; try (intro X; inversion X). 
+        assumption.
+      (* and the interesting part of the invariant is preserved: *)
+        (* X has to be a cons *)
+        destruct (aslist (st X)) as [|h x'] eqn:Heqx.
+          unfold bassn in H9. unfold beval in H9. unfold aeval in H9. 
+          rewrite -> Heqx in H9. inversion H9.
+
+          exists (snoc p h).
+          split.
+            rewrite update_eq.
+            unfold aeval. rewrite -> Heqx.
+            rewrite snoc_equation. assumption.
+
+            rewrite update_neq; try (intro X; inversion X). 
+            split.
+              intros. apply appears_in_snoc2. apply H3. assumption.
+
+              intros.  destruct (appears_in_snoc3 _ _ _ H).
+              SCase "later".
+                inversion H3 as [_ H3'].
+                apply H3'. assumption.
+              SCase "here (absurd)".
+                subst.
+                unfold bassn, beval, aeval in H10.
+                rewrite not_true_iff_false in H10.
+                apply beq_nat_false in H10. 
+                rewrite -> Heqx in H10. simpl in H10.
+                apply ex_falso_quodlibet. apply H10. assumption.
+  (* The invariant holds at the start of the loop: *)
+  intros st [H1 [H2 H3]]. 
+  rewrite H1. rewrite H2. rewrite H3.
+  split. 
+    reflexivity.
+    exists []. split.
+      reflexivity.
+      split; intros H; inversion H.
+  (* At the end of the loop the invariant implies the right thing. *)
+  simpl.   intros st [[H1 [p [H2 H3]]] H5].
+  (* x must be [] *)
+  unfold bassn in H5. unfold beval in H5. unfold aeval in H5.
+  destruct (aslist (st X)) as [|h x'].
+    rewrite append_nil in H2.
+    rewrite <- H2.
+    assumption.
+
+    apply ex_falso_quodlibet. apply H5. reflexivity.
+Qed.
+
+Fixpoint rev {X:Type} (l:list X) : list X :=
+  match l with
+  | nil => []
+  | cons h t => snoc (rev t) h
+  end.
+
+Definition list_reverse_program :=
+  Y ::= ANil;
+  WHILE (BIsCons (AId X)) DO
+    Y ::= ACons (AHead (AId X)) (AId Y);
+    X ::= ATail (AId X)
+  END.
+
+Lemma rev_equation : forall (A : Type) (h : A) (x y : list A),
+  rev (h :: x) ++ y = rev x ++ h :: y.
+Proof.
+  intros. simpl. apply snoc_equation.
+Qed.
+
+Theorem list_rev_correct : forall l,
+  {{ fun st => aslist (st X) =  l }}
+    list_reverse_program
+  {{ fun st => aslist (st Y) = rev l }}.
+Proof.
+  intros.
+  destruct (eq_id_dec X Y) eqn:eqxy; try inversion eqxy.
+    unfold list_reverse_program.
+    eapply hoare_seq.
+      eapply hoare_consequence_post with (fun st : state => rev(aslist (st X)) ++ aslist (st Y) = rev l /\ ~ bassn (BIsCons (AId X)) st).
+        apply hoare_while.
+        eapply hoare_consequence_pre.
+          eapply hoare_seq.
+            apply hoare_asgn.
+            apply hoare_asgn.
+          intros st [H0 H1]. inversion H1.
+          destruct (st X) eqn:stx. inversion H2.
+          destruct l0. inversion H2.
+          simpl in H0.
+          unfold assn_sub. simpl. rewrite stx.
+          simpl.
+          rewrite update_neq; auto. rewrite stx. simpl.
+          rewrite <- rev_equation. simpl. assumption.
+        intros st [H0 H1].
+          destruct (st X) eqn:stx. simpl in H0. assumption.
+          destruct l0. simpl in H0. assumption.
+          assert(H:False); try inversion H. apply H1. unfold bassn.
+          simpl. rewrite stx. reflexivity.
+      eapply hoare_consequence_post with (fun st : state => aslist (st X) = l /\ aslist (st Y) = []).
+        eapply hoare_consequence_pre.
+        apply hoare_asgn.
+        unfold assn_sub. simpl. intros st H. split; auto.
+        intros st [H0 H1]. destruct (st Y) eqn:sty; subst; simpl. apply append_nil.
+        simpl in H1. rewrite H1. apply append_nil.
+  Qed.
+
+Inductive dcom : Type :=
+  | DCSkip :  Assertion -> dcom
+  | DCSeq : dcom -> dcom -> dcom
+  | DCAsgn : id -> aexp ->  Assertion -> dcom
+  | DCIf : bexp ->  Assertion -> dcom ->  Assertion -> dcom
+           -> Assertion-> dcom
+  | DCWhile : bexp -> Assertion -> dcom -> Assertion -> dcom
+  | DCPre : Assertion -> dcom -> dcom
+  | DCPost : dcom -> Assertion -> dcom.
+
+Tactic Notation "dcom_cases" tactic(first) ident(c) :=
+  first;
+  [ Case_aux c "Skip" | Case_aux c "Seq" | Case_aux c "Asgn"
+  | Case_aux c "If" | Case_aux c "While"
+  | Case_aux c "Pre" | Case_aux c "Post" ].
+
+Notation "'SKIP' {{ P }}" 
+      := (DCSkip P) 
+      (at level 10) : dcom_scope.
+Notation "l '::=' a {{ P }}" 
+      := (DCAsgn l a P) 
+      (at level 60, a at next level) : dcom_scope.
+Notation "'WHILE' b 'DO' {{ Pbody }} d 'END' {{ Ppost }}" 
+      := (DCWhile b Pbody d Ppost) 
+      (at level 80, right associativity) : dcom_scope.
+Notation "'IFB' b 'THEN' {{ P }} d 'ELSE' {{ P' }} d' 'FI' {{ Q }}" 
+      := (DCIf b P d P' d' Q) 
+      (at level 80, right associativity)  : dcom_scope.
+Notation "'=>' {{ P }} d" 
+      := (DCPre P d) 
+      (at level 90, right associativity)  : dcom_scope.
+Notation "{{ P }} d" 
+      := (DCPre P d) 
+      (at level 90)  : dcom_scope.
+Notation "d '=>' {{ P }}" 
+      := (DCPost d P) 
+      (at level 91, right associativity)  : dcom_scope.
+Notation " d ; d' " 
+      := (DCSeq d d') 
+      (at level 80, right associativity)  : dcom_scope.
+
+Delimit Scope dcom_scope with dcom.
+
+Example dec_while : dcom := (
+  {{ fun st => True }}
+  WHILE (BNot (BEq (AId X) (ANum 0))) 
+  DO
+    {{ fun st => True /\ bassn (BNot (BEq (AId X) (ANum 0))) st}}
+    X ::= (AMinus (AId X) (ANum 1)) 
+    {{ fun _ => True }}
+  END
+  {{ fun st => True /\ ~bassn (BNot (BEq (AId X) (ANum 0))) st}} =>
+  {{ fun st => asnat (st X) = 0 }}
+) % dcom.
+
+Fixpoint extract (d:dcom) : com :=
+  match d with
+  | DCSkip _           => SKIP
+  | DCSeq d1 d2        => (extract d1 ; extract d2) 
+  | DCAsgn X a _       => X ::= a
+  | DCIf b _ d1 _ d2 _ => IFB b THEN extract d1 ELSE extract d2 FI
+  | DCWhile b _ d _    => WHILE b DO extract d END
+  | DCPre _ d          => extract d
+  | DCPost d _         => extract d
+  end.
+
+Fixpoint post (d:dcom) : Assertion :=
+  match d with
+  | DCSkip P                => P
+  | DCSeq d1 d2             => post d2
+  | DCAsgn X a Q            => Q
+  | DCIf  _ _ d1 _ d2 Q     => Q
+  | DCWhile b Pbody c Ppost => Ppost
+  | DCPre _ d               => post d
+  | DCPost c Q              => Q
+  end.
+
+Fixpoint pre (d:dcom) : Assertion :=
+  match d with
+  | DCSkip P                => fun st => True
+  | DCSeq c1 c2             => pre c1
+  | DCAsgn X a Q            => fun st => True
+  | DCIf  _ _ t _ e _       => fun st => True
+  | DCWhile b Pbody c Ppost => fun st => True
+  | DCPre P c               => P
+  | DCPost c Q              => pre c
+  end.
+
+Definition dec_correct (d:dcom) := 
+  {{pre d}} (extract d) {{post d}}.
+
+Fixpoint verification_conditions (P : Assertion) (d:dcom) : Prop :=
+  match d with
+  | DCSkip Q          => 
+      (P ->> Q)
+  | DCSeq d1 d2      => 
+      verification_conditions P d1
+      /\ verification_conditions (post d1) d2
+  | DCAsgn X a Q      => 
+      (P ->> assn_sub X a Q)
+  | DCIf b P1 d1 P2 d2 Q => 
+      ((fun st => P st /\ bassn b st) ->> P1)
+      /\ ((fun st => P st /\ ~ (bassn b st)) ->> P2)
+      /\ (Q = post d1) /\ (Q = post d2)
+      /\ verification_conditions P1 d1
+      /\ verification_conditions P2 d2
+  | DCWhile b Pbody d Ppost      => 
+      (* post d is the loop invariant and the initial precondition *)
+      (P ->> post d)  
+      /\ (Pbody = (fun st => post d st /\ bassn b st))
+      /\ (Ppost = (fun st => post d st /\ ~(bassn b st)))
+      /\ verification_conditions Pbody d
+  | DCPre P' d         => 
+      (P ->> P') /\ verification_conditions P' d
+  | DCPost d Q        => 
+      verification_conditions P d /\ (post d ->> Q)
+  end.
+
+Theorem verification_correct : forall d P, 
+  verification_conditions P d -> {{P}} (extract d) {{post d}}.
+Proof.
+  dcom_cases (induction d) Case; intros P H; simpl in *.
+  Case "Skip".
+    eapply hoare_consequence_pre.
+      apply hoare_skip.
+      assumption.
+  Case "Seq". 
+    inversion H as [H1 H2]. clear H. 
+    eapply hoare_seq. 
+      apply IHd2. apply H2.
+      apply IHd1. apply H1.
+  Case "Asgn". 
+    eapply hoare_consequence_pre.
+      apply hoare_asgn.
+      assumption.
+  Case "If".
+    inversion H as [HPre1 [HPre2 [Hd1 [Hd2 [HThen HElse]]]]]; clear H.
+    subst.
+    apply hoare_if.
+      eapply hoare_consequence_pre. apply IHd1. eassumption. assumption.
+      rewrite Hd2.
+      eapply hoare_consequence_pre. apply IHd2. eassumption. assumption.
+  Case "While".
+    inversion H as [Hpre [Hbody [Hpost Hd]]]; subst; clear H.
+    eapply hoare_consequence_pre.
+    apply hoare_while with (P := post d). 
+      apply IHd. apply Hd. 
+      assumption.
+  Case "Pre".
+    inversion H as [HP Hd]; clear H. 
+    eapply hoare_consequence_pre. apply IHd. apply Hd. assumption.
+  Case "Post".
+    inversion H as [Hd HQ]; clear H.
+    eapply hoare_consequence_post. apply IHd. apply Hd. assumption.
+Qed.
+
+Tactic Notation "verify" :=
+  try apply verification_correct; 
+  repeat split;
+  simpl; unfold assert_implies; 
+  unfold bassn in *; unfold beval in *; unfold aeval in *;
+  unfold assn_sub; intros;
+  repeat rewrite update_eq;
+  repeat (rewrite update_neq; [| (intro X; inversion X)]);
+  simpl in *; 
+  repeat match goal with [H : _ /\ _ |- _] => destruct H end;
+  repeat rewrite not_true_iff_false in *;
+  repeat rewrite not_false_iff_true in *;
+  repeat rewrite negb_true_iff in *;
+  repeat rewrite negb_false_iff in *;
+  repeat rewrite beq_nat_true_iff in *;
+  repeat rewrite beq_nat_false_iff in *;
+  try eauto; try omega.
+
+Definition list_member_dec (n : nat) (l : list nat) : dcom := (
+    {{ fun st => aslist (st X) = l /\ asnat (st Y) = n /\ asnat (st Z) = 0 }}
+  WHILE BIsCons (AId X)
+  DO {{ fun st => (asnat (st Y) = n 
+               /\ (exists p, p ++ aslist (st X) = l 
+               /\ (asnat (st Z) = 1 <-> appears_in n p)))
+               /\ bassn (BIsCons (AId X)) st }}
+    IFB (BEq (AId Y) (AHead (AId X))) THEN
+        {{ fun st =>
+          ((asnat (st Y) = n 
+            /\ (exists p, p ++ aslist (st X) = l 
+                /\ (asnat (st Z) = 1 <-> appears_in n p)))
+          /\ bassn (BIsCons (AId X)) st)
+          /\ bassn (BEq (AId Y) (AHead (AId X))) st }}
+        =>
+        {{ fun st => 
+            asnat (st Y) = n 
+            /\ (exists p, p ++ tail (aslist (st X)) = l 
+                 /\ (1 = 1 <-> appears_in n p)) }}
+      Z ::= ANum 1
+        {{ fun st => asnat (st Y) = n 
+             /\ (exists p, p ++ tail (aslist (st X)) = l 
+                  /\ (asnat (st Z) = 1 <-> appears_in n p)) }}
+   ELSE
+        {{ fun st =>
+          ((asnat (st Y) = n 
+            /\ (exists p, p ++ aslist (st X) = l 
+                  /\ (asnat (st Z) = 1 <-> appears_in n p)))
+          /\ bassn (BIsCons (AId X)) st)
+          /\ ~bassn (BEq (AId Y) (AHead (AId X))) st }}
+        =>
+        {{ fun st => 
+          asnat (st Y) = n 
+          /\ (exists p, p ++ tail (aslist (st X)) = l 
+               /\ (asnat (st Z) = 1 <-> appears_in n p)) }}
+      SKIP
+        {{ fun st => asnat (st Y) = n 
+            /\ (exists p, p ++ tail (aslist (st X)) = l 
+                 /\ (asnat (st Z) = 1 <-> appears_in n p)) }}
+   FI
+     {{ fun st => asnat (st Y) = n 
+        /\ (exists p, p ++ tail (aslist (st X)) = l 
+          /\ (asnat (st Z) = 1 <-> appears_in n p)) }}
+   ;
+   X ::= (ATail (AId X))
+     {{ fun st  =>
+         asnat (st Y) = n /\
+         (exists p : list nat, p ++ aslist (st X) = l 
+           /\ (asnat (st Z) = 1 <-> appears_in n p)) }}
+  END
+   {{ fun st =>
+     (asnat (st Y) = n 
+       /\ (exists p, p ++ aslist (st X) = l 
+            /\ (asnat (st Z) = 1 <-> appears_in n p)))
+     /\ ~bassn (BIsCons (AId X)) st }}
+   =>
+   {{ fun st => asnat (st Z) = 1 <-> appears_in n l }}
+) %dcom.
+
+Theorem list_member_correct' : forall n l,
+  dec_correct (list_member_dec n l).
+Proof.
+  intros n l. verify.
+  Case "The loop precondition holds.".
+    exists []. simpl. split.
+      rewrite H. reflexivity.
+      rewrite H1. split; intro Hc; inversion Hc.
+  Case "IF taken".
+    destruct H2 as [p [H3 H4]].
+    (* We know X is non-nil. *)
+    destruct (aslist (st X)) as [|h x'].
+      inversion H1.
+      exists (snoc p h).
+      simpl. split.
+         rewrite snoc_equation. assumption.
+         split.
+           rewrite H in H0.
+           simpl in H0. rewrite H0.
+           intros _. apply appears_in_snoc1.
+           intros _. reflexivity.
+  Case "If not taken".
+    destruct H2 as [p [H3 H4]].
+    (* We know X is non-nil. *)
+    destruct (aslist (st X)) as [|h x'].
+      inversion H1.
+      exists (snoc p h).
+      split. simpl.
+        rewrite snoc_equation. assumption.
+        split.
+          intros. apply appears_in_snoc2. apply H4. assumption.
+          intros Hai.  destruct (appears_in_snoc3 _ _ _ Hai).
+          SCase "later". apply H4. assumption.
+          SCase "here (absurd)".
+            subst. simpl in H0. 
+            apply ex_falso_quodlibet. apply H0. assumption.
+  Case "Loop postcondition implies desired conclusion (->)".
+    destruct H2 as [p [H3 H4]].
+    destruct (aslist (st X)) as [|h x'].
+       rewrite append_nil in H3. subst. apply H4. assumption.
+       inversion H1.
+  Case "loop postcondition implies desired conclusion (<-)".
+    destruct H2 as [p [H3 H4]].
+    destruct (aslist (st X)) as [|h x'].
+       rewrite append_nil in H3. subst. apply H4. assumption.
+       inversion H1.
+Qed.
