Rel.v
@@ -1,0 +1,235 @@
+Add LoadPath "D:\sfsol".
+Require Export SfLib.
+
+Definition relation (X: Type) := X->X->Prop.
+
+Print le.
+
+Check le : nat->nat->Prop.
+
+Check le : relation nat.
+
+Definition partial_function {X: Type} (R: relation X) :=
+  forall x y1 y2 : X, R x y1 -> R x y2 -> y1 = y2.
+
+Theorem le_not_a_partial_function :
+  ~ (partial_function le).
+Proof.
+  unfold not. unfold partial_function. intros Hc.
+  assert (0 = 1) as Nonsense.
+   Case "Proof of assertion".
+   apply Hc with (x := 0).
+     apply le_n.
+     apply le_S. apply le_n.
+  inversion Nonsense. Qed.
+
+Inductive total_relation : nat -> nat -> Prop :=
+  | total : forall n1 n2, total_relation n1 n2.
+
+Inductive empty_relation : nat -> nat -> Prop :=
+  | empty : forall n1 n2, 0 = 1 -> empty_relation n1 n2.
+
+Theorem total_not_a_partial_function :
+  ~ (partial_function total_relation).
+Proof.
+  unfold not. unfold partial_function. intros.
+  assert (0 = 1) as Nonsense.
+  apply H with 0; constructor. inversion Nonsense.
+  Qed.
+
+Theorem empty_not_a_partial_function :
+  (partial_function empty_relation).
+Proof.
+  unfold partial_function. intros.
+  inversion H. inversion H1. Qed.
+
+Definition reflexive {X: Type} (R: relation X) :=
+  forall a : X, R a a.
+
+Theorem le_reflexive :
+  reflexive le.
+Proof.
+  unfold reflexive. intros n. apply le_n. Qed.
+
+Definition transitive {X: Type} (R: relation X) :=
+  forall a b c : X, (R a b) -> (R b c) -> (R a c).
+
+Theorem le_trans :
+  transitive le.
+Proof.
+  intros n m o Hnm Hmo.
+  induction Hmo.
+  Case "le_n". apply Hnm.
+  Case "le_S". apply le_S. apply IHHmo. Qed.
+
+Theorem lt_trans:
+  transitive lt.
+Proof.
+  unfold lt. unfold transitive.
+  intros n m o Hnm Hmo.
+  apply le_S in Hnm.
+  apply le_trans with (a := (S n)) (b := (S m)) (c := o).
+  apply Hnm.
+  apply Hmo. Qed.
+
+Theorem lt_trans' :
+  transitive lt.
+Proof.
+  unfold lt. unfold transitive.
+  intros n m o Hnm Hmo.
+  induction Hmo as [| m' Hm'o].
+    apply le_S. assumption.
+    apply le_S. assumption.
+  Qed.
+
+Theorem le_Sn_le : forall n m, S n <= m -> n <= m.
+Proof.
+  intros n m H. apply le_trans with (S n).
+    apply le_S. apply le_n.
+    apply H. Qed.
+
+Theorem le_S_n : forall n m,
+  (S n <= S m) -> (n <= m).
+Proof.
+  intros. generalize dependent n. induction m.
+  intros. inversion H; try constructor. inversion H1.
+  intros. inversion H; try constructor. apply IHm.
+  assumption.
+  Qed.
+
+Theorem le_Sn_n : forall n,
+  ~ (S n <= n).
+Proof.
+  induction n.
+  intros H. inversion H.
+  intros H. apply IHn. apply le_S_n.
+  assumption.
+  Qed.
+
+Definition symmetric {X: Type} (R: relation X) :=
+  forall a b : X, (R a b) -> (R b a).
+
+Theorem le_not_symmetric :
+  ~ (symmetric le).
+Proof.
+  unfold symmetric. intros H.
+  assert(1<=0). apply H. constructor.
+  constructor. inversion H0.
+  Qed.
+
+Definition antisymmetric {X: Type} (R: relation X) :=
+  forall a b : X, (R a b) -> (R b a) -> a = b.
+
+Theorem le_antisymmetric :
+  antisymmetric le.
+Proof.
+  intros a b H1 H2.
+  generalize dependent b. induction a; intros.
+  inversion H2. reflexivity.
+  destruct b. inversion H1.
+  apply le_S_n in H1. apply le_S_n in H2.
+  replace a with b. reflexivity.
+  symmetry. apply IHa; assumption.
+  Qed.
+
+Theorem le_step : forall n m p,
+  n < m ->
+  m <= S p ->
+  n <= p.
+Proof.
+  intros.
+  unfold lt in H.
+  apply le_S_n. eapply le_trans.
+  apply H. apply H0.
+  Qed.
+
+Definition equivalence {X:Type} (R: relation X) :=
+  (reflexive R) /\ (symmetric R) /\ (transitive R).
+
+Definition order {X:Type} (R: relation X) :=
+  (reflexive R) /\ (antisymmetric R) /\ (transitive R).
+
+Definition preorder {X:Type} (R: relation X) :=
+  (reflexive R) /\ (transitive R).
+
+Theorem le_order :
+  order le.
+Proof.
+  unfold order. split.
+    Case "refl". apply le_reflexive.
+    split.
+      Case "antisym". apply le_antisymmetric.
+      Case "transitive.". apply le_trans. Qed.
+
+Inductive clos_refl_trans {A: Type} (R: relation A) : relation A :=
+    | rt_step : forall x y, R x y -> clos_refl_trans R x y
+    | rt_refl : forall x, clos_refl_trans R x x
+    | rt_trans : forall x y z,
+          clos_refl_trans R x y ->
+          clos_refl_trans R y z ->
+          clos_refl_trans R x z.
+
+Theorem next_nat_closure_is_le : forall n m,
+  (n <= m) <-> ((clos_refl_trans next_nat) n m).
+Proof.
+  intros n m. split.
+    Case "->".
+      intro H. induction H.
+      SCase "le_n". apply rt_refl.
+      SCase "le_S".
+        apply rt_trans with m. apply IHle. apply rt_step. apply nn.
+    Case "<-".
+      intro H. induction H.
+      SCase "rt_step". inversion H. apply le_S. apply le_n.
+      SCase "rt_refl". apply le_n.
+      SCase "rt_trans".
+        apply le_trans with y.
+        apply IHclos_refl_trans1.
+        apply IHclos_refl_trans2. Qed.
+
+Inductive refl_step_closure {X:Type} (R: relation X) : relation X :=
+  | rsc_refl : forall (x : X), refl_step_closure R x x
+  | rsc_step : forall (x y z : X),
+                    R x y ->
+                    refl_step_closure R y z ->
+                    refl_step_closure R x z.
+
+Tactic Notation "rt_cases" tactic(first) ident(c) :=
+  first;
+  [ Case_aux c "rt_step" | Case_aux c "rt_refl"
+  | Case_aux c "rt_trans" ].
+
+Tactic Notation "rsc_cases" tactic(first) ident(c) :=
+  first;
+  [ Case_aux c "rsc_refl" | Case_aux c "rsc_step" ].
+
+Theorem rsc_R : forall (X:Type) (R:relation X) (x y : X),
+       R x y -> refl_step_closure R x y.
+Proof.
+  intros X R x y H.
+  apply rsc_step with y. apply H. apply rsc_refl. Qed.
+
+Theorem rsc_trans :
+  forall (X:Type) (R: relation X) (x y z : X),
+      refl_step_closure R x y ->
+      refl_step_closure R y z ->
+      refl_step_closure R x z.
+Proof.
+  intros.
+  induction H. assumption.
+  eapply rsc_step. apply H.
+  apply IHrefl_step_closure. assumption.
+  Qed.
+
+Theorem rtc_rsc_coincide :
+         forall (X:Type) (R: relation X) (x y : X),
+  clos_refl_trans R x y <-> refl_step_closure R x y.
+Proof.
+  split; intros; induction H.
+    eapply rsc_step. apply H. apply rsc_refl.
+    apply rsc_refl. apply rsc_trans with y; auto.
+  apply rt_refl.
+    apply rt_trans with y.
+      apply rt_step; assumption.
+      assumption.
+  Qed.
