Smallstep.v
@@ -1,0 +1,346 @@
+Add LoadPath "D:\sfsol".
+Require Export Imp.
+
+Definition relation (X: Type) := X->X->Prop.
+
+Inductive tm : Type :=
+  | C : nat -> tm
+  | P : tm -> tm -> tm.
+
+Tactic Notation "tm_cases" tactic(first) ident(c) :=
+  first;
+  [ Case_aux c "C" | Case_aux c "P" ].
+
+Fixpoint evalF (t : tm) : nat :=
+  match t with
+  | C n => n
+  | P a1 a2 => evalF a1 + evalF a2
+  end.
+
+Reserved Notation " t '||' n " (at level 50, left associativity).
+
+Inductive eval : tm -> nat -> Prop :=
+  | E_Const : forall n,
+      C n || n
+  | E_Plus : forall t1 t2 n1 n2,
+      t1 || n1 ->
+      t2 || n2 ->
+      P t1 t2 || (n1 + n2)
+
+  where " t '||' n " := (eval t n).
+
+Tactic Notation "eval_cases" tactic(first) ident(c) :=
+  first;
+  [ Case_aux c "E_Const" | Case_aux c "E_Plus" ].
+
+Module SimpleArith1.
+
+Reserved Notation " t '=>' t' " (at level 40).
+
+Inductive step : tm -> tm -> Prop :=
+  | ST_PlusConstConst : forall n1 n2,
+      P (C n1) (C n2) => C (n1 + n2)
+  | ST_Plus1 : forall t1 t1' t2,
+      t1 => t1' ->
+      P t1 t2 => P t1' t2
+  | ST_Plus2 : forall n1 t2 t2',
+      t2 => t2' ->
+      P (C n1) t2 => P (C n1) t2'
+
+  where " t '=>' t' " := (step t t').
+
+Tactic Notation "step_cases" tactic(first) ident(c) :=
+  first;
+  [ Case_aux c "ST_PlusConstConst"
+  | Case_aux c "ST_Plus1" | Case_aux c "ST_Plus2" ].
+
+Example test_step_1 :
+      P
+        (P (C 0) (C 3))
+        (P (C 2) (C 4))
+      =>
+      P
+        (C (0 + 3))
+        (P (C 2) (C 4)).
+Proof. apply ST_Plus1. apply ST_PlusConstConst.
+  Qed.
+
+Example test_step_2 :
+      P
+        (C 0)
+        (P
+          (C 2)
+          (P (C 0) (C 3)))
+      =>
+      P
+        (C 0)
+        (P
+          (C 2)
+          (C (0 + 3))).
+Proof. apply ST_Plus2. apply ST_Plus2. apply ST_PlusConstConst.
+  Qed.
+
+Definition deterministic {X: Type} (R: relation X) :=
+  forall x y1 y2 : X, R x y1 -> R x y2 -> y1 = y2.
+
+Theorem step_deterministic:
+  deterministic step.
+Proof.
+  intros x y z H1 H2. generalize dependent z.
+  induction H1; intros. inversion H2. reflexivity. inversion H3. inversion H3.
+  inversion H2. rewrite <- H0 in H1. inversion H1.
+  replace (t1'0) with t1'. reflexivity. apply IHstep. assumption. rewrite <- H in H1.
+  inversion H1. inversion H2; subst. inversion H1. inversion H4. replace (t2'0) with t2'.
+  reflexivity. apply IHstep. apply H4.
+  Qed.
+
+End SimpleArith1.
+
+Inductive value : tm -> Prop :=
+  v_const : forall n, value (C n).
+
+Reserved Notation " t '=>' t' " (at level 40).
+
+Inductive step : tm -> tm -> Prop :=
+  | ST_PlusConstConst : forall n1 n2,
+          P (C n1) (C n2)
+      => C (n1 + n2)
+  | ST_Plus1 : forall t1 t1' t2,
+        t1 => t1' ->
+        P t1 t2 => P t1' t2
+  | ST_Plus2 : forall v1 t2 t2',
+        value v1 ->
+        t2 => t2' ->
+        P v1 t2 => P v1 t2'
+
+  where " t '=>' t' " := (step t t').
+
+Tactic Notation "step_cases" tactic(first) ident(c) :=
+  first;
+  [ Case_aux c "ST_PlusConstConst"
+  | Case_aux c "ST_Plus1" | Case_aux c "ST_Plus2" ].
+
+Theorem step_deterministic :
+  deterministic step.
+Proof.
+  intros x y z H. generalize dependent z.
+  induction H; intros. inversion H; subst. reflexivity. inversion H3. inversion H4.
+  inversion H0; subst. inversion H. replace t1'0 with t1'. reflexivity. apply IHstep. assumption.
+  inversion H; subst; inversion H3.
+  inversion H1; subst. inversion H0. inversion H5; subst; inversion H.
+  replace t2'0 with t2'. reflexivity. apply IHstep. assumption.
+  Qed.
+
+Theorem strong_progress : forall t,
+  value t \/ (exists t', t => t').
+Proof.
+  induction t.
+  apply or_introl; constructor.
+  apply or_intror; inversion IHt1.
+  inversion IHt2; inversion H; inversion H0.
+  apply ex_intro with (C (n + n0)). constructor.
+  apply ex_intro with (P (C n) x). repeat constructor. assumption.
+  inversion H. apply ex_intro with (P x t2). constructor. assumption.
+  Qed.
+
+Definition normal_form {X:Type} (R:relation X) (t:X) : Prop :=
+  ~ exists t', R t t'.
+
+Lemma value_is_nf : forall v,
+  value v -> normal_form step v.
+Proof.
+  intros. unfold normal_form. unfold not. intros.
+  inversion H0. inversion H1; subst; inversion H.
+  Qed.
+
+Lemma nf_is_value : forall t,
+  normal_form step t -> value t.
+Proof.
+  intros. destruct t. constructor.
+  assert(H0:(value (P t1 t2)) \/ ((exists t', (P t1 t2) => t'))); try inversion H0; try assumption.
+    apply strong_progress.
+  assert(contra:False);try inversion contra. apply H. assumption.
+  Qed.
+
+Corollary nf_same_as_value : forall t,
+  normal_form step t <-> value t.
+Proof.
+  split. apply nf_is_value. apply value_is_nf. Qed.
+
+Module Temp1.
+
+Inductive value : tm -> Prop :=
+| v_const : forall n, value (C n)
+| v_funny : forall t1 n2,
+              value (P t1 (C n2)).
+
+Reserved Notation " t '=>' t' " (at level 40).
+
+Inductive step : tm -> tm -> Prop :=
+  | ST_PlusConstConst : forall n1 n2,
+      P (C n1) (C n2) => C (n1 + n2)
+  | ST_Plus1 : forall t1 t1' t2,
+      t1 => t1' ->
+      P t1 t2 => P t1' t2
+  | ST_Plus2 : forall v1 t2 t2',
+      value v1 ->
+      t2 => t2' ->
+      P v1 t2 => P v1 t2'
+
+  where " t '=>' t' " := (step t t').
+
+Lemma value_not_same_as_normal_form :
+  exists v, value v /\ ~ normal_form step v.
+Proof.
+  exists (P (C 0) (C 0)). split. constructor.
+  intros H. apply H. exists (C 0). constructor.
+  Qed.
+
+End Temp1.
+
+Module Temp2.
+
+Inductive value : tm -> Prop :=
+| v_const : forall n, value (C n).
+
+Reserved Notation " t '=>' t' " (at level 40).
+
+Inductive step : tm -> tm -> Prop :=
+  | ST_Funny : forall n,
+      C n => P (C n) (C 0)
+  | ST_PlusConstConst : forall n1 n2,
+      P (C n1) (C n2) => C (n1 + n2)
+  | ST_Plus1 : forall t1 t1' t2,
+      t1 => t1' ->
+      P t1 t2 => P t1' t2
+  | ST_Plus2 : forall v1 t2 t2',
+      value v1 ->
+      t2 => t2' ->
+      P v1 t2 => P v1 t2'
+
+  where " t '=>' t' " := (step t t').
+
+Lemma value_not_same_as_normal_form :
+  exists v, value v /\ ~ normal_form step v.
+Proof.
+  exists (C 0). split. constructor.
+  intros H; apply H. exists (P (C 0) (C 0)).
+  constructor.
+  Qed.
+
+End Temp2.
+
+Module Temp3.
+
+Inductive value : tm -> Prop :=
+  | v_const : forall n, value (C n).
+
+Reserved Notation " t '=>' t' " (at level 40).
+
+Inductive step : tm -> tm -> Prop :=
+  | ST_PlusConstConst : forall n1 n2,
+      P (C n1) (C n2) => C (n1 + n2)
+  | ST_Plus1 : forall t1 t1' t2,
+      t1 => t1' ->
+      P t1 t2 => P t1' t2
+
+  where " t '=>' t' " := (step t t').
+
+Lemma value_not_same_as_normal_form :
+  exists t, ~ value t /\ normal_form step t.
+Proof.
+  exists (P (C 0) (P (C 0) (C 0))). split;
+  intros H. inversion H. inversion H.
+  inversion H0; subst. inversion H4.
+  Qed.
+
+End Temp3.
+
+Module Temp4.
+
+Inductive tm : Type :=
+  | ttrue : tm
+  | tfalse : tm
+  | tif : tm -> tm -> tm -> tm.
+
+Inductive value : tm -> Prop :=
+  | v_true : value ttrue
+  | v_false : value tfalse.
+
+Reserved Notation " t '=>' t' " (at level 40).
+
+Inductive step : tm -> tm -> Prop :=
+  | ST_IfTrue : forall t1 t2,
+      tif ttrue t1 t2 => t1
+  | ST_IfFalse : forall t1 t2,
+      tif tfalse t1 t2 => t2
+  | ST_If : forall t1 t1' t2 t3,
+      t1 => t1' ->
+      tif t1 t2 t3 => tif t1' t2 t3
+
+  where " t '=>' t' " := (step t t').
+
+Definition bool_step_prop1 :=
+  tfalse => tfalse.
+
+Theorem neg_bool_step_prop1 :
+  ~ bool_step_prop1.
+Proof.
+  intros H. inversion H. Qed.
+
+Definition bool_step_prop2 :=
+     tif
+       ttrue
+       (tif ttrue ttrue ttrue)
+       (tif tfalse tfalse tfalse)
+  =>
+     ttrue.
+
+Theorem neg_bool_step_prop2 :
+  ~ bool_step_prop2.
+Proof.
+  intros H. inversion H. Qed.
+
+Definition bool_step_prop3 :=
+     tif
+       (tif ttrue ttrue ttrue)
+       (tif ttrue ttrue ttrue)
+       tfalse
+   =>
+     tif
+       ttrue
+       (tif ttrue ttrue ttrue)
+       tfalse.
+
+Theorem neg_bool_step_prop3 :
+  bool_step_prop3.
+Proof.
+  constructor. constructor. Qed.
+
+Theorem strong_progress : forall t,
+  value t \/ (exists t', t => t').
+Proof.
+  induction t.
+    apply or_introl; constructor.
+    apply or_introl; constructor.
+    apply or_intror.
+      inversion IHt1; inversion H; subst.
+      exists t2; constructor.
+      exists t3; constructor.
+      exists (tif x t2 t3); constructor. assumption.
+  Qed.
+
+Theorem step_deterministic :
+  deterministic step.
+Proof.
+  intros x y z H. generalize dependent z.
+  induction H; intros.
+  inversion H; subst; try reflexivity; try inversion H4.
+  inversion H; subst; try reflexivity; try inversion H4.
+  inversion H0; subst. inversion H. inversion H.
+  replace t1'0 with t1'. reflexivity.
+  apply IHstep. assumption.
+  Qed.
+
+Module Temp5.
+
